WIP:Proving the elimination of Pallocframe

x86/Asm.v
@@ -1512,6 +1512,13 @@ Qed.
 
 End INSTRSIZE.
 
+(** instrsize instantiation *)
+Definition instr_size_1 (i:Asm.instruction) : Z := 1.
+Lemma instr_size_bound_1 : forall i, 0 < instr_size_1 i <= Ptrofs.max_unsigned.
+Proof.
+  intros. destruct i; simpl; vm_compute; split; congruence.
+Qed.
+
 (** Classification functions for processor registers (used in Asmgenproof). *)
 
 Definition data_preg (r: preg) : bool :=
